code/bignum/Hacl.Impl.MultiExponentiation.fsti
@@ -137,3 +137,164 @@ val lexp_double_fw_consttime:
   -> k:concrete_ops a_t len ctx_len
   -> l:size_window_t a_t len ->
   lexp_double_fw_st a_t len ctx_len k l
+
+//--------------------------------------------------
+
+inline_for_extraction noextract
+let lexp_four_fw_tables_st
+  (a_t:inttype_a)
+  (len:size_t{v len > 0})
+  (ctx_len:size_t)
+  (k:concrete_ops a_t len ctx_len)
+  (l:size_window_t a_t len)
+  (table_len:table_len_t len)
+  (table_inv1:table_inv_t a_t len table_len)
+  (table_inv2:table_inv_t a_t len table_len)
+  (table_inv3:table_inv_t a_t len table_len)
+  (table_inv4:table_inv_t a_t len table_len)
+  =
+    ctx:lbuffer (uint_t a_t SEC) ctx_len
+  -> a1:lbuffer (uint_t a_t SEC) len
+  -> bLen:size_t
+  -> bBits:size_t{(v bBits - 1) / bits a_t < v bLen}
+  -> b1:lbuffer (uint_t a_t SEC) bLen
+  -> a2:lbuffer (uint_t a_t SEC) len
+  -> b2:lbuffer (uint_t a_t SEC) bLen
+  -> a3:lbuffer (uint_t a_t SEC) len
+  -> b3:lbuffer (uint_t a_t SEC) bLen
+  -> a4:lbuffer (uint_t a_t SEC) len
+  -> b4:lbuffer (uint_t a_t SEC) bLen
+  -> table1:lbuffer (uint_t a_t SEC) (table_len *! len)
+  -> table2:lbuffer (uint_t a_t SEC) (table_len *! len)
+  -> table3:lbuffer (uint_t a_t SEC) (table_len *! len)
+  -> table4:lbuffer (uint_t a_t SEC) (table_len *! len)
+  -> res:lbuffer (uint_t a_t SEC) len ->
+  Stack unit
+  (requires fun h ->
+    live h a1 /\ live h b1 /\ live h a2 /\ live h b2 /\
+    live h a3 /\ live h b3 /\ live h a4 /\ live h b4 /\
+    live h res /\ live h ctx /\
+    live h table1 /\ live h table2 /\ live h table3 /\ live h table4 /\
+
+    eq_or_disjoint a1 a2 /\ eq_or_disjoint a1 a3 /\ eq_or_disjoint a1 a4 /\
+    eq_or_disjoint a2 a3 /\ eq_or_disjoint a2 a4 /\ eq_or_disjoint a3 a4 /\
+    disjoint a1 res /\ disjoint a1 ctx /\ disjoint a2 res /\ disjoint a2 ctx /\
+    disjoint a3 res /\ disjoint a3 ctx /\ disjoint a4 res /\ disjoint a4 ctx /\
+    disjoint b1 res /\ disjoint b2 res /\ disjoint b3 res /\ disjoint b4 res /\
+    disjoint res ctx /\ disjoint res table1 /\ disjoint res table2 /\
+    disjoint res table3 /\ disjoint res table4 /\
+
+    BD.bn_v h b1 < pow2 (v bBits) /\
+    BD.bn_v h b2 < pow2 (v bBits) /\
+    BD.bn_v h b3 < pow2 (v bBits) /\
+    BD.bn_v h b4 < pow2 (v bBits) /\
+    k.to.linv_ctx (as_seq h ctx) /\
+    k.to.linv (as_seq h a1) /\ k.to.linv (as_seq h a2) /\
+    k.to.linv (as_seq h a3) /\ k.to.linv (as_seq h a4) /\
+    table_inv1 (as_seq h a1) (as_seq h table1) /\
+    table_inv2 (as_seq h a2) (as_seq h table2) /\
+    table_inv3 (as_seq h a3) (as_seq h table3) /\
+    table_inv4 (as_seq h a4) (as_seq h table4))
+  (ensures  fun h0 _ h1 -> modifies (loc res) h0 h1 /\
+    k.to.linv (as_seq h1 res) /\
+    k.to.refl (as_seq h1 res) ==
+    S.exp_four_fw k.to.comm_monoid
+      (k.to.refl (as_seq h0 a1)) (v bBits) (BD.bn_v h0 b1)
+      (k.to.refl (as_seq h0 a2)) (BD.bn_v h0 b2)
+      (k.to.refl (as_seq h0 a3)) (BD.bn_v h0 b3)
+      (k.to.refl (as_seq h0 a4)) (BD.bn_v h0 b4) (v l))
+
+
+inline_for_extraction noextract
+val mk_lexp_four_fw_tables:
+    #a_t:inttype_a
+  -> len:size_t{v len > 0}
+  -> ctx_len:size_t
+  -> k:concrete_ops a_t len ctx_len
+  -> l:size_window_t a_t len
+  -> table_len:table_len_t len
+  -> table_inv1:table_inv_t a_t len table_len
+  -> table_inv2:table_inv_t a_t len table_len
+  -> table_inv3:table_inv_t a_t len table_len
+  -> table_inv4:table_inv_t a_t len table_len
+  -> pow_a_to_small_b1:pow_a_to_small_b_st a_t len ctx_len k l table_len table_inv1
+  -> pow_a_to_small_b2:pow_a_to_small_b_st a_t len ctx_len k l table_len table_inv2
+  -> pow_a_to_small_b3:pow_a_to_small_b_st a_t len ctx_len k l table_len table_inv3
+  -> pow_a_to_small_b4:pow_a_to_small_b_st a_t len ctx_len k l table_len table_inv4 ->
+  lexp_four_fw_tables_st a_t len ctx_len k l table_len table_inv1 table_inv2 table_inv3 table_inv4
+
+
+// Fixed-window method with four precomputed tables
+// table1 = [a1^0 = one; a1^1; a1^2; ..; a1^(table_len - 1)]
+// table2 = [a2^0 = one; a2^1; a2^2; ..; a2^(table_len - 1)]
+// table3 = [a3^0 = one; a3^1; a3^2; ..; a3^(table_len - 1)]
+// table4 = [a4^0 = one; a4^1; a4^2; ..; a4^(table_len - 1)]
+//-----------------------------------------------------------
+
+inline_for_extraction noextract
+let lexp_four_fw_st
+  (a_t:inttype_a)
+  (len:size_t{v len > 0})
+  (ctx_len:size_t)
+  (k:concrete_ops a_t len ctx_len)
+  (l:size_window_t a_t len) =
+    ctx:lbuffer (uint_t a_t SEC) ctx_len
+  -> a1:lbuffer (uint_t a_t SEC) len
+  -> bLen:size_t
+  -> bBits:size_t{(v bBits - 1) / bits a_t < v bLen}
+  -> b1:lbuffer (uint_t a_t SEC) bLen
+  -> a2:lbuffer (uint_t a_t SEC) len
+  -> b2:lbuffer (uint_t a_t SEC) bLen
+  -> a3:lbuffer (uint_t a_t SEC) len
+  -> b3:lbuffer (uint_t a_t SEC) bLen
+  -> a4:lbuffer (uint_t a_t SEC) len
+  -> b4:lbuffer (uint_t a_t SEC) bLen
+  -> res:lbuffer (uint_t a_t SEC) len ->
+  Stack unit
+  (requires fun h ->
+    live h a1 /\ live h b1 /\ live h a2 /\ live h b2 /\
+    live h a3 /\ live h b3 /\ live h a4 /\ live h b4 /\
+    live h res /\ live h ctx /\
+
+    eq_or_disjoint a1 a2 /\ eq_or_disjoint a1 a3 /\ eq_or_disjoint a1 a4 /\
+    eq_or_disjoint a2 a3 /\ eq_or_disjoint a2 a4 /\ eq_or_disjoint a3 a4 /\
+    disjoint a1 res /\ disjoint a1 ctx /\ disjoint a2 res /\ disjoint a2 ctx /\
+    disjoint a3 res /\ disjoint a3 ctx /\ disjoint a4 res /\ disjoint a4 ctx /\
+    disjoint b1 res /\ disjoint b2 res /\ disjoint b3 res /\ disjoint b4 res /\
+    disjoint res ctx /\
+
+    BD.bn_v h b1 < pow2 (v bBits) /\
+    BD.bn_v h b2 < pow2 (v bBits) /\
+    BD.bn_v h b3 < pow2 (v bBits) /\
+    BD.bn_v h b4 < pow2 (v bBits) /\
+    k.to.linv_ctx (as_seq h ctx) /\
+    k.to.linv (as_seq h a1) /\ k.to.linv (as_seq h a2) /\
+    k.to.linv (as_seq h a3) /\ k.to.linv (as_seq h a4))
+  (ensures  fun h0 _ h1 -> modifies (loc res) h0 h1 /\
+    k.to.linv (as_seq h1 res) /\
+    k.to.refl (as_seq h1 res) ==
+    S.exp_four_fw k.to.comm_monoid
+      (k.to.refl (as_seq h0 a1)) (v bBits) (BD.bn_v h0 b1)
+      (k.to.refl (as_seq h0 a2)) (BD.bn_v h0 b2)
+      (k.to.refl (as_seq h0 a3)) (BD.bn_v h0 b3)
+      (k.to.refl (as_seq h0 a4)) (BD.bn_v h0 b4) (v l))
+
+
+inline_for_extraction noextract
+val lexp_four_fw_vartime:
+    #a_t:inttype_a
+  -> len:size_t{v len > 0}
+  -> ctx_len:size_t
+  -> k:concrete_ops a_t len ctx_len
+  -> l:size_window_t a_t len ->
+  lexp_four_fw_st a_t len ctx_len k l
+
+
+inline_for_extraction noextract
+val lexp_four_fw_consttime:
+    #a_t:inttype_a
+  -> len:size_t{v len > 0}
+  -> ctx_len:size_t
+  -> k:concrete_ops a_t len ctx_len
+  -> l:size_window_t a_t len ->
+  lexp_four_fw_st a_t len ctx_len k l
